src/hls/GiblePargenproofBackward.v
@@ -76,15 +76,41 @@ Definition remember_expr (f : forest) (lst: list pred_expr) (i : instr): list pr
   | RBexit p c => lst
   end.
 
+Definition remember_expr_inc (fop : pred_op * forest) (lst: list pred_expr) (i : instr): list pred_expr :=
+  let (pred, f) := fop in
+  match i with
+  | RBnop => lst
+  | RBop p op rl r => (app_predicated (dfltp p ∧ pred) (NE.singleton (Ptrue, Ebase (Reg 1))) (
+        (seq_app (pred_ret (Eop op)) (merge (list_translation rl f))))) :: lst
+  | RBload p chunk addr rl r => (app_predicated (dfltp p ∧ pred) (NE.singleton (Ptrue, Ebase (Reg 1))) (
+        (seq_app
+          (seq_app (pred_ret (Eload chunk addr))
+            (merge (list_translation rl f)))
+            (f #r Mem)))) :: lst
+  | RBstore p chunk addr rl r => lst
+  | RBsetpred p' c args p =>  lst
+  | RBexit p c => lst
+  end.
+
 Definition update' (s: pred_op * forest * list pred_expr * list pred_expr) (i: instr): option (pred_op * forest * list pred_expr * list pred_expr) :=
   let '(p, f, l, lm) := s in
   Option.bind2 (fun p' f' => Option.ret (p', f', remember_expr f l i, remember_expr_m f lm i)) (update (p, f) i).
+
+Definition update'_inc (s: pred_op * forest * list pred_expr * list pred_expr) (i: instr): option (pred_op * forest * list pred_expr * list pred_expr) :=
+  let '(p, f, l, lm) := s in
+  Option.bind2 (fun p' f' => Option.ret (p', f', remember_expr_inc (p, f) l i, remember_expr_m_inc (p, f) lm i)) (update (p, f) i).
 
 Definition abstract_sequence' (b : list instr) : option (forest * list pred_expr * list pred_expr) :=
   Option.bind (fun x => Option.bind (fun _ => Some x)
     (mfold_left gather_predicates b (Some (PTree.empty _))))
       (Option.map (fun x => let '(_, y, z, zm) := x in (y, z, zm))
         (mfold_left update' b (Some (Ptrue, empty, nil, nil)))).
+
+Definition abstract_sequence'_inc (b : list instr) : option (forest * list pred_expr * list pred_expr) :=
+  Option.bind (fun x => Option.bind (fun _ => Some x)
+    (mfold_left gather_predicates b (Some (PTree.empty _))))
+      (Option.map (fun x => let '(_, y, z, zm) := x in (y, z, zm))
+        (mfold_left update'_inc b (Some (Ptrue, empty, nil, nil)))).
 
 Section CORRECTNESS.
 
@@ -106,12 +132,34 @@ Proof.
     eapply IHi; eauto.
 Qed.
 
+Lemma equiv_update_inc:
+  forall i p f l lm p' f' l' lm',
+    mfold_left update'_inc i (Some (p, f, l, lm)) = Some (p', f', l', lm') ->
+    mfold_left update i (Some (p, f)) = Some (p', f').
+Proof.
+  induction i; cbn -[update] in *; intros.
+  - inv H; auto.
+  - exploit OptionExtra.mfold_left_Some; eauto;
+      intros [[[[p_mid f_mid] l_mid] lm_mid] HB].
+    unfold Option.bind2, Option.ret in HB; repeat destr. inv Heqp1.
+    eapply IHi; eauto.
+Qed.
+
 Lemma equiv_update1:
   forall i p f l lm p' f' l' lm',
     update' (p, f, l, lm) i = Some (p', f', l', lm') ->
     update (p, f) i = Some (p', f').
 Proof.
   intros. unfold update', Option.bind2, Option.ret in *. repeat destr.
+  now inv H.
+Qed.
+
+Lemma equiv_update1_inc:
+  forall i p f l lm p' f' l' lm',
+    update'_inc (p, f, l, lm) i = Some (p', f', l', lm') ->
+    update (p, f) i = Some (p', f').
+Proof.
+  intros. unfold update'_inc, Option.bind2, Option.ret in *. repeat destr.
   now inv H.
 Qed.
 
@@ -147,6 +195,18 @@ Definition evaluable_pred_expr {G} (ctx: @Abstr.ctx G) pr p :=
 
 Definition evaluable_pred_expr_m {G} (ctx: @Abstr.ctx G) pr p :=
   exists r, sem_pred_expr pr sem_mem ctx p r.
+
+Definition cond_evaluable_pred_expr {G} (ctx: @Abstr.ctx G) pr ps cond p :=
+  eval_predf ps cond = true ->
+  exists r, sem_pred_expr pr sem_value ctx p r.
+
+Definition cond_evaluable_pred_expr_m {G} (ctx: @Abstr.ctx G) pr ps cond p :=
+  eval_predf ps cond = true ->
+  exists r, sem_pred_expr pr sem_mem ctx p r.
+
+Definition evaluable_forest {G} (ctx: @Abstr.ctx G) pr f := 
+  (forall x, evaluable_pred_expr ctx pr (f #r (Reg x)))
+  /\ evaluable_pred_expr_m ctx pr (f #r Mem).
 
 Definition evaluable_pred_list {G} ctx pr l :=
   forall p,
@@ -472,11 +532,25 @@ Proof.
   unfold remember_expr; destruct a; eauto using in_cons.
 Qed.
 
+Lemma remember_expr_in_inc :
+  forall x l f a,
+    In x l -> In x (remember_expr_inc f l a).
+Proof.
+  unfold remember_expr_inc; destruct a; repeat destruct_match; eauto using in_cons.
+Qed.
+
 Lemma remember_expr_in_m :
   forall x l f a,
     In x l -> In x (remember_expr_m f l a).
 Proof.
-  unfold remember_expr; destruct a; eauto using in_cons.
+  unfold remember_expr_m; destruct a; eauto using in_cons.
+Qed.
+
+Lemma remember_expr_in_m_inc :
+  forall x l f a,
+    In x l -> In x (remember_expr_m_inc f l a).
+Proof.
+  unfold remember_expr_m_inc; destruct a; repeat destruct_match; eauto using in_cons.
 Qed.
 
 Lemma in_mfold_left_abstr :
@@ -495,6 +569,22 @@ Proof.
     auto using remember_expr_in.
 Qed.
 
+Lemma in_mfold_left_abstr_inc :
+  forall instrs p f l p' f' l' x lm lm',
+    mfold_left update'_inc instrs (Some (p, f, l, lm)) = Some (p', f', l', lm') ->
+    In x l -> In x l'.
+Proof.
+  induction instrs; intros.
+  - cbn in *; now inv H.
+  - cbn -[update] in *.
+    pose proof H as Y.
+    apply OptionExtra.mfold_left_Some in Y. inv Y.
+    rewrite H1 in H. destruct x0 as (((p_int & f_int) & l_int) & lm_int).
+    exploit IHinstrs; eauto.
+    unfold Option.bind2, Option.ret in H1; repeat destr. inv H1.
+    destruct a; auto; apply in_cons; auto.
+Qed.
+
 Lemma in_mfold_left_abstr_m :
   forall instrs p f l p' f' l' x lm lm',
     mfold_left update' instrs (Some (p, f, l, lm)) = Some (p', f', l', lm') ->
@@ -509,6 +599,22 @@ Proof.
     exploit IHinstrs; eauto.
     unfold Option.bind2, Option.ret in H1; repeat destr. inv H1.
     auto using remember_expr_in_m.
+Qed.
+
+Lemma in_mfold_left_abstr_m_inc:
+  forall instrs p f l p' f' l' x lm lm',
+    mfold_left update'_inc instrs (Some (p, f, l, lm)) = Some (p', f', l', lm') ->
+    In x lm -> In x lm'.
+Proof.
+  induction instrs; intros.
+  - cbn in *; now inv H.
+  - cbn -[update remember_expr_inc remember_expr_m_inc] in *.
+    pose proof H as Y.
+    apply OptionExtra.mfold_left_Some in Y. inv Y.
+    rewrite H1 in H. destruct x0 as (((p_int & f_int) & l_int) & lm_int).
+    exploit IHinstrs; eauto.
+    unfold Option.bind, Option.bind2, Option.ret in *; repeat destr. inv H1.
+    destruct a; auto. apply in_cons; auto.
 Qed.
 
 Lemma not_remembered_in_forest :
@@ -614,6 +720,34 @@ Proof.
   inv H0. inv H5. rewrite H2.
   unfold evaluable_pred_expr_m. eauto.
 Qed.
+
+(* Lemma in_forest_evaluable_inc : *)
+(*   forall G sp ge i' cf instrs p f l p' f' l' x i0 lm lm', *)
+(*     mfold_left update'_inc instrs (Some (p, f, l, lm)) = Some (p', f', l', lm') -> *)
+(*     sem (mk_ctx i0 sp ge) f' (i', cf) -> *)
+(*     @evaluable_pred_list G (mk_ctx i0 sp ge) f'.(forest_preds) l' -> *)
+(*     evaluable_pred_expr (mk_ctx i0 sp ge) f'.(forest_preds) (f #r (Reg x)). *)
+(* Proof. *)
+(*   intros. *)
+(*   pose proof H as Y. apply in_forest_or_remembered with (x := x) in Y. *)
+(*   inv Y; eauto. *)
+(*   inv H0. inv H5. rewrite H2. *)
+(*   unfold evaluable_pred_expr. eauto. *)
+(* Qed. *)
+
+(* Lemma in_forest_evaluable_m_inc : *)
+(*   forall G sp ge i' cf instrs p f l p' f' l' i0 lm lm', *)
+(*     mfold_left update'_inc instrs (Some (p, f, l, lm)) = Some (p', f', l', lm') -> *)
+(*     sem (mk_ctx i0 sp ge) f' (i', cf) -> *)
+(*     @evaluable_pred_list_m G (mk_ctx i0 sp ge) f'.(forest_preds) lm' -> *)
+(*     evaluable_pred_expr_m (mk_ctx i0 sp ge) f'.(forest_preds) (f #r Mem). *)
+(* Proof. *)
+(*   intros. *)
+(*   pose proof H as Y. apply in_forest_or_remembered_m in Y. *)
+(*   inv Y; eauto. *)
+(*   inv H0. inv H5. rewrite H2. *)
+(*   unfold evaluable_pred_expr_m. eauto. *)
+(* Qed. *)
 
 Definition pe_preds_in {A} (x: predicated A) preds :=
   NE.Forall (fun x => forall pred, PredIn pred (fst x)
@@ -1346,6 +1480,20 @@ Proof.
   eapply abstr_seq_revers_correct_fold_sem_pexpr_eval3''; eauto.
 Qed.
 
+Lemma abstr_seq_revers_correct_fold_sem_pexpr_eval3'_inc :
+  forall A B G a_sem instrs p f p' f' i0 sp ge preds preds' pe pe_val l l' lm lm',
+    update'_inc (p, f, l, lm) instrs = Some (p', f', l', lm') ->
+    gather_predicates preds instrs = Some preds' ->
+    @sem_pred_expr G A B f'.(forest_preds) a_sem (mk_ctx i0 sp ge) pe pe_val ->
+    NE.Forall (fun x => forall pred, PredIn pred (fst x) -> preds ! pred = Some tt) pe ->
+    sem_pred_expr f.(forest_preds) a_sem (mk_ctx i0 sp ge) pe pe_val.
+Proof.
+  intros.
+  unfold update'_inc, Option.bind2, Option.ret in H; repeat destr.
+  inversion H; subst.
+  eapply abstr_seq_revers_correct_fold_sem_pexpr_eval3''; eauto.
+Qed.
+
 Lemma abstr_seq_revers_correct_fold_sem_pexpr_eval3 :
   forall A B G a_sem instrs p f l p' f' l' i0 sp ge preds preds' pe pe_val lm lm',
     mfold_left update' instrs (Some (p, f, l, lm)) = Some (p', f', l', lm') ->
@@ -1369,6 +1517,29 @@ Proof.
   eapply abstr_seq_revers_correct_fold_sem_pexpr_eval3'; eauto.
 Qed.
 
+Lemma abstr_seq_revers_correct_fold_sem_pexpr_eval3_inc :
+  forall A B G a_sem instrs p f l p' f' l' i0 sp ge preds preds' pe pe_val lm lm',
+    mfold_left update'_inc instrs (Some (p, f, l, lm)) = Some (p', f', l', lm') ->
+    mfold_left gather_predicates instrs (Some preds) = Some preds' ->
+    @sem_pred_expr G A B f'.(forest_preds) a_sem (mk_ctx i0 sp ge) pe pe_val ->
+    NE.Forall (fun x => forall pred, PredIn pred (fst x) -> preds ! pred = Some tt) pe ->
+    sem_pred_expr f.(forest_preds) a_sem (mk_ctx i0 sp ge) pe pe_val.
+Proof.
+  induction instrs; [crush|].
+  intros. cbn -[update remember_expr_inc remember_expr_m_inc] in H,H0.
+  exploit OptionExtra.mfold_left_Some. eapply H. intros [[[[p_mid f_mid] l_mid] lm_mid] HBind].
+  rewrite HBind in H.
+  exploit OptionExtra.mfold_left_Some. eapply H0. intros [preds_mid HGATHER].
+  rewrite HGATHER in H0.
+  exploit IHinstrs; eauto.
+  apply NE.Forall_forall. intros [p_op aval] YIN ypred YPREDIN.
+  apply NE.Forall_forall with (x:=(p_op, aval)) in H2; auto. cbn [fst snd] in *.
+  specialize (H2 ypred YPREDIN).
+  eapply gather_predicates_in; eassumption.
+  intros HSEM.
+  eapply abstr_seq_revers_correct_fold_sem_pexpr_eval3'_inc; eauto.
+Qed.
+
 Lemma abstr_seq_revers_correct_fold_sem_pexpr_eval2 :
   forall G instrs p f l p' f' l' i0 sp ge preds preds' pe lm lm',
     mfold_left update' instrs (Some (p, f, l, lm)) = Some (p', f', l', lm') ->
@@ -1381,6 +1552,20 @@ Proof.
   unfold evaluable_pred_expr in *.
   intros. inv H1. exists x.
   eapply abstr_seq_revers_correct_fold_sem_pexpr_eval3; eauto.
+Qed.
+
+Lemma abstr_seq_revers_correct_fold_sem_pexpr_eval2_inc :
+  forall G instrs p f l p' f' l' i0 sp ge preds preds' pe lm lm',
+    mfold_left update'_inc instrs (Some (p, f, l, lm)) = Some (p', f', l', lm') ->
+    mfold_left gather_predicates instrs (Some preds) = Some preds' ->
+    @evaluable_pred_expr G (mk_ctx i0 sp ge) f'.(forest_preds) pe ->
+    NE.Forall (fun x => forall pred, PredIn pred (fst x)
+                 -> PTree.get pred preds = Some tt) pe ->
+    evaluable_pred_expr (mk_ctx i0 sp ge) f.(forest_preds) pe.
+Proof.
+  unfold evaluable_pred_expr in *.
+  intros. inv H1. exists x.
+  eapply abstr_seq_revers_correct_fold_sem_pexpr_eval3_inc; eauto.
 Qed.
 
 Lemma abstr_seq_revers_correct_fold_sem_pexpr_eval4 :
@@ -1397,6 +1582,20 @@ Proof.
   eapply abstr_seq_revers_correct_fold_sem_pexpr_eval3; eauto.
 Qed.
 
+Lemma abstr_seq_revers_correct_fold_sem_pexpr_eval4_inc :
+  forall G instrs p f l p' f' l' i0 sp ge preds preds' pe lm lm',
+    mfold_left update'_inc instrs (Some (p, f, l, lm)) = Some (p', f', l', lm') ->
+    mfold_left gather_predicates instrs (Some preds) = Some preds' ->
+    @evaluable_pred_expr_m G (mk_ctx i0 sp ge) f'.(forest_preds) pe ->
+    NE.Forall (fun x => forall pred, PredIn pred (fst x)
+                 -> PTree.get pred preds = Some tt) pe ->
+    evaluable_pred_expr_m (mk_ctx i0 sp ge) f.(forest_preds) pe.
+Proof.
+  unfold evaluable_pred_expr in *.
+  intros. inv H1. exists x.
+  eapply abstr_seq_revers_correct_fold_sem_pexpr_eval3_inc; eauto.
+Qed.
+
 Lemma state_lessdef_state_equiv :
   forall x y, state_lessdef x y <-> state_equiv x y.
 Proof. split; intros; inv H; constructor; auto. Qed.
@@ -1404,6 +1603,24 @@ Proof. split; intros; inv H; constructor; auto. Qed.
 Lemma abstr_seq_revers_correct_fold_sem_pexpr :
   forall instrs p f l p' f' l' preds preds' lm lm',
     mfold_left update' instrs (Some (p, f, l, lm)) = Some (p', f', l', lm') ->
+    mfold_left gather_predicates instrs (Some preds) = Some preds' ->
+    forall pred, preds ! pred = Some tt ->
+      f #p pred = f' #p pred.
+Proof.
+  induction instrs; try solve [crush].
+  intros. cbn -[update] in *.
+  exploit OptionExtra.mfold_left_Some. apply H. intros [[[[p_mid f_mid] l_mid] lm_mid] HBIND].
+  exploit OptionExtra.mfold_left_Some. apply H0. intros [ptree_mid HGATHER].
+  rewrite HBIND in H. rewrite HGATHER in H0.
+  exploit IHinstrs; eauto. eapply gather_predicates_in; eauto.
+  intros. rewrite <- H2.
+  unfold "#p". unfold get_forest_p'. erewrite abstr_seq_revers_correct_fold_sem_pexpr_sem2; eauto.
+  unfold Option.bind2, Option.ret in *. repeat destr. inv Heqp1. inv HBIND. eauto.
+Qed.
+
+Lemma abstr_seq_revers_correct_fold_sem_pexpr_inc :
+  forall instrs p f l p' f' l' preds preds' lm lm',
+    mfold_left update'_inc instrs (Some (p, f, l, lm)) = Some (p', f', l', lm') ->
     mfold_left gather_predicates instrs (Some preds) = Some preds' ->
     forall pred, preds ! pred = Some tt ->
       f #p pred = f' #p pred.
@@ -1463,6 +1680,60 @@ Lemma update_rev_gather_constant2:
     (forall p, preds' ! p = None -> sem_pexpr (mk_ctx i0 sp ge) (f' #p p) ps).
 Proof.
   unfold update', gather_predicates; destruct i; intros; unfold Option.bind, Option.bind2, Option.ret in *;
+    repeat destr.
+  - inv H0. inv H1. inv Heqo. eauto.
+  - inv H0. cbn in *. unfold Option.bind, Option.bind2, Option.ret in *;
+    repeat destr; inv Heqo1; inv H4. destruct o. inv H1. eapply gather_predicates_fold3 in H2. eauto. inv H1; eauto.
+  - inv H0. cbn in *. unfold Option.bind, Option.bind2, Option.ret in *;
+    repeat destr; inv Heqo1; inv H4. inv Heqo0. destruct o. inv H1. eapply gather_predicates_fold3 in H2.
+    eauto. inv H1; eauto.
+  - inv H0. cbn in *. unfold Option.bind, Option.bind2, Option.ret in *;
+    repeat destr; inv Heqo1; inv H4. inv Heqo0. destruct o. inv H1. eapply gather_predicates_fold3 in H2.
+    eauto. inv H1; eauto.
+  - inv H0. cbn in *. unfold Option.bind, Option.bind2, Option.ret in *. repeat destr. inv Heqo1. inv H4.
+    destruct (peq p1 p); subst. inv H1. rewrite PTree.gss in H2. discriminate.
+    rewrite forest_pred_gso by auto. inv H1. rewrite PTree.gso in H2 by auto.
+    destruct o. eapply gather_predicates_fold3 in H2. eauto. eauto.
+  - inv H0. cbn in *. unfold Option.bind, Option.bind2, Option.ret in *;
+    repeat destr; inv Heqo1; inv H4. inv Heqo0. destruct o. inv H1. eapply gather_predicates_fold3 in H2.
+    eauto. inv H1; eauto.
+Qed.
+
+Lemma update_rev_gather_constant_inc:
+  forall G i preds i0 sp ge f p l lm p' f' l' lm' preds' ps,
+    (forall p, preds ! p = None -> @sem_pexpr G (mk_ctx i0 sp ge) (f #p p) (ps !! p)) ->
+    update'_inc (p, f, l, lm) i = Some (p', f', l', lm') ->
+    gather_predicates preds i = Some preds' ->
+    (forall p, preds' ! p = None -> sem_pexpr (mk_ctx i0 sp ge) (f' #p p) (ps !! p)).
+Proof.
+  unfold update'_inc, gather_predicates; destruct i; intros; unfold Option.bind, Option.bind2, Option.ret in *;
+    repeat destr.
+  - inv H0. inv H1. inv Heqo. eauto.
+  - inv H0. cbn in *. unfold Option.bind, Option.bind2, Option.ret in *;
+    repeat destr; inv Heqo1; inv H4. destruct o. inv H1. eapply gather_predicates_fold3 in H2. eauto. inv H1; eauto.
+  - inv H0. cbn in *. unfold Option.bind, Option.bind2, Option.ret in *;
+    repeat destr; inv Heqo1; inv H4. inv Heqo0. destruct o. inv H1. eapply gather_predicates_fold3 in H2.
+    eauto. inv H1; eauto.
+  - inv H0. cbn in *. unfold Option.bind, Option.bind2, Option.ret in *;
+    repeat destr; inv Heqo1; inv H4. inv Heqo0. destruct o. inv H1. eapply gather_predicates_fold3 in H2.
+    eauto. inv H1; eauto.
+  - inv H0. cbn in *. unfold Option.bind, Option.bind2, Option.ret in *. repeat destr. inv Heqo1. inv H4.
+    destruct (peq p1 p); subst. inv H1. rewrite PTree.gss in H2. discriminate.
+    rewrite forest_pred_gso by auto. inv H1. rewrite PTree.gso in H2 by auto.
+    destruct o. eapply gather_predicates_fold3 in H2. eauto. eauto.
+  - inv H0. cbn in *. unfold Option.bind, Option.bind2, Option.ret in *;
+    repeat destr; inv Heqo1; inv H4. inv Heqo0. destruct o. inv H1. eapply gather_predicates_fold3 in H2.
+    eauto. inv H1; eauto.
+Qed.
+
+Lemma update_rev_gather_constant2_inc:
+  forall G i preds i0 sp ge f p l lm p' f' l' lm' preds' ps,
+    (forall p, preds ! p = None -> @sem_pexpr G (mk_ctx i0 sp ge) (f #p p) ps) ->
+    update'_inc (p, f, l, lm) i = Some (p', f', l', lm') ->
+    gather_predicates preds i = Some preds' ->
+    (forall p, preds' ! p = None -> sem_pexpr (mk_ctx i0 sp ge) (f' #p p) ps).
+Proof.
+  unfold update'_inc, gather_predicates; destruct i; intros; unfold Option.bind, Option.bind2, Option.ret in *;
     repeat destr.
   - inv H0. inv H1. inv Heqo. eauto.
   - inv H0. cbn in *. unfold Option.bind, Option.bind2, Option.ret in *;
@@ -1571,6 +1842,57 @@ Proof.
     exploit OptionExtra.mfold_left_Some. apply H0. intros [ptree_mid HGATHER].
     rewrite HBIND in H. rewrite HGATHER in H0.
     exploit IHinstrs. 3: { eauto. } 3: { eauto. } eapply update_rev_gather_constant; eauto.
+    eauto. eauto.
+    intros [ps_mid HSEM_MID].
+    (* destruct (preds ! p0) eqn:?. destruct u. eapply gather_predicates_in in HGATHER; eauto. *)
+    (* rewrite HGATHER in H2. discriminate. *)
+    unfold Option.bind2, Option.bind, Option.ret in *; repeat destr. inv HBIND.
+    destruct a; cbn in *.
+    + inv Heqo. inv HGATHER. eauto.
+    + unfold Option.bind2, Option.bind, Option.ret in *; repeat destr.
+      generalize dependent Heqo; repeat destr; intros Heqo; inv Heqo.
+      inv HSEM_MID.
+      econstructor. constructor; eauto.
+    + unfold Option.bind2, Option.bind, Option.ret in *; repeat destr.
+      generalize dependent Heqo; repeat destr; intros Heqo; inv Heqo.
+      inv HSEM_MID.
+      econstructor. constructor; eauto.
+    + unfold Option.bind2, Option.bind, Option.ret in *; repeat destr.
+      generalize dependent Heqo; repeat destr; intros Heqo; inv Heqo.
+      inv HSEM_MID.
+      econstructor. constructor; eauto.
+    + unfold Option.bind2, Option.bind, Option.ret in *; repeat destr. inv HGATHER.
+      generalize dependent Heqo; repeat destr; intros Heqo; inv Heqo.
+      exists (mask_pred_map preds (is_ps i0) ps_mid).
+      econstructor; intros.
+      destruct (peq x p0); subst.
+      * destruct o; [assert (YX: preds ! p0 = None) by (eapply gather_predicates_fold3; eauto)|];
+          rewrite mask_pred_map_not_in_pred; auto.
+      * inv HSEM_MID. specialize (H2 x). rewrite forest_pred_gso in H2 by auto.
+        destruct (preds ! x) eqn:HDESTR.
+        -- destruct u3. now rewrite mask_pred_map_in_pred.
+        -- rewrite mask_pred_map_not_in_pred; auto.
+    + unfold Option.bind2, Option.bind, Option.ret in *; repeat destr.
+      generalize dependent Heqo; repeat destr; intros Heqo; inv Heqo.
+      inv HSEM_MID.
+      econstructor. constructor; eauto.
+Qed.
+
+Lemma abstr_seq_revers_correct_fold_sem_pexpr_eval_inc :
+  forall G instrs p f l p' f' l' i0 sp ge preds preds' ps' lm lm',
+    (forall p, preds ! p = None -> sem_pexpr (mk_ctx i0 sp ge) (f #p p) ((is_ps i0) !! p)) ->
+    mfold_left update'_inc instrs (Some (p, f, l, lm)) = Some (p', f', l', lm') ->
+    mfold_left gather_predicates instrs (Some preds) = Some preds' ->
+    sem_predset (@mk_ctx G i0 sp ge) f' ps' ->
+    exists ps, sem_predset (mk_ctx i0 sp ge) f ps.
+Proof.
+  induction instrs.
+  - intros * YH **. cbn in *. inv H. inv H0. eauto.
+  - intros * YH **. cbn -[update remember_expr_inc remember_expr_m_inc] in *.
+    exploit OptionExtra.mfold_left_Some. apply H. intros [[[[p_mid f_mid] l_mid] lm_mid] HBIND].
+    exploit OptionExtra.mfold_left_Some. apply H0. intros [ptree_mid HGATHER].
+    rewrite HBIND in H. rewrite HGATHER in H0.
+    exploit IHinstrs. 3: { eauto. } 3: { eauto. } eapply update_rev_gather_constant_inc; eauto.
     eauto. eauto.
     intros [ps_mid HSEM_MID].
     (* destruct (preds ! p0) eqn:?. destruct u. eapply gather_predicates_in in HGATHER; eauto. *)
@@ -1795,6 +2117,346 @@ Proof.
         Unshelve. all: exact nil.
 Qed.
 
+Lemma eval_app_predicated :
+  forall G (ctx: @Abstr.ctx G) (a b: predicated expression) p f_p ps c,
+    (forall x0 : positive, sem_pexpr ctx (get_forest_p' x0 f_p) ps !! x0) ->
+    evaluable_pred_expr ctx f_p (app_predicated p c a) ->
+    evaluable_pred_expr ctx f_p b ->
+    evaluable_pred_expr ctx f_p (app_predicated p b a).
+Proof.
+  intros * HPred HEvalR HEvalL.
+  inv HEvalR. inv HEvalL.
+  case_eq (eval_predf ps p); intros.
+  - exists x. apply sem_pred_expr_app_predicated with (ps:=ps); auto.
+    eapply sem_pred_expr_app_predicated2; eauto.
+  - exists x0. apply sem_pred_expr_app_predicated_false with (ps:=ps); auto.
+Qed.
+
+Lemma eval_prune_predicated :
+  forall G (ctx: @Abstr.ctx G) (a b: predicated expression) f_p ps,
+    (forall x0 : positive, sem_pexpr ctx (get_forest_p' x0 f_p) ps !! x0) ->
+    prune_predicated a = Some b ->
+    evaluable_pred_expr ctx f_p a ->
+    evaluable_pred_expr ctx f_p b.
+Proof.
+  intros * HPred Hprune HEval. inv HEval.
+  exists x. eapply sem_pred_expr_prune_predicated; eauto.
+Qed.
+
+Lemma eval_app_predicated_m :
+  forall G (ctx: @Abstr.ctx G) (a b: predicated expression) p f_p ps c,
+    (forall x0 : positive, sem_pexpr ctx (get_forest_p' x0 f_p) ps !! x0) ->
+    evaluable_pred_expr_m ctx f_p (app_predicated p c a) ->
+    evaluable_pred_expr_m ctx f_p b ->
+    evaluable_pred_expr_m ctx f_p (app_predicated p b a).
+Proof.
+  intros * HPred HEvalR HEvalL.
+  inv HEvalR. inv HEvalL.
+  case_eq (eval_predf ps p); intros.
+  - exists x. apply sem_pred_expr_app_predicated with (ps:=ps); auto.
+    eapply sem_pred_expr_app_predicated2; eauto.
+  - exists x0. apply sem_pred_expr_app_predicated_false with (ps:=ps); auto.
+Qed.
+
+Lemma eval_prune_predicated_m :
+  forall G (ctx: @Abstr.ctx G) (a b: predicated expression) f_p ps,
+    (forall x0 : positive, sem_pexpr ctx (get_forest_p' x0 f_p) ps !! x0) ->
+    prune_predicated a = Some b ->
+    evaluable_pred_expr_m ctx f_p a ->
+    evaluable_pred_expr_m ctx f_p b.
+Proof.
+  intros * HPred Hprune HEval. inv HEval.
+  exists x. eapply sem_pred_expr_prune_predicated; eauto.
+Qed.
+
+Lemma eval_forest_update_inc :
+  forall sp i i0 p p' f f' l l' lm lm' f_p ps,
+    (forall x0 : positive, sem_pexpr (mk_ctx i0 sp ge) (get_forest_p' x0 f_p) ps !! x0) ->
+    update'_inc (p, f, l, lm) i = Some (p', f', l', lm') ->
+    evaluable_pred_list (mk_ctx i0 sp ge) f_p l' ->
+    evaluable_pred_list_m (mk_ctx i0 sp ge) f_p lm' ->
+    evaluable_forest (mk_ctx i0 sp ge) f_p f ->
+    evaluable_forest (mk_ctx i0 sp ge) f_p f'.
+Proof.
+  destruct i; intros * Hpred **; cbn -[app_predicated seq_app] in *; unfold Option.ret, Option.bind2, Option.bind in *; repeat (destruct_match; try easy; []).
+  - inv H; auto.
+  - inv H. inv Heqo1. inv H2.
+    constructor.
+    2: {
+      inv H3. exists x. rewrite forest_reg_gso by discriminate. auto.
+    }
+    intro x. destruct (peq x r); subst.
+    2: {
+      rewrite forest_reg_gso; auto. unfold not; intros. inv H2. contradiction.
+    }
+    rewrite forest_reg_gss.
+    unfold evaluable_pred_list in *.
+    exploit eval_app_predicated. eauto. eapply H0. constructor. eauto.
+    eapply H. instantiate (1:=r). intros.
+    eapply eval_prune_predicated; eauto.
+  - inv H. inv Heqo0. inv H2.
+    constructor.
+    2: {
+      inv H3. exists x. rewrite forest_reg_gso by discriminate. auto.
+    }
+    intro x. destruct (peq x r); subst.
+    2: {
+      rewrite forest_reg_gso; auto. unfold not; intros. inv H2. contradiction.
+    }
+    rewrite forest_reg_gss.
+    unfold evaluable_pred_list in *.
+    exploit eval_app_predicated. eauto. eapply H0. constructor. eauto.
+    eapply H. instantiate (1:=r). intros.
+    eapply eval_prune_predicated; eauto.
+  - inv Heqo0. inv H. inv H2.
+    constructor; intros.
+    rewrite forest_reg_gso by discriminate. auto.
+    rewrite forest_reg_gss. 
+    exploit eval_app_predicated_m. eauto. apply H1. constructor. eauto.
+    apply H3.
+    intros. eapply eval_prune_predicated_m; eauto.
+  - inv Heqo0. inv H. inv H2. constructor; intros; rewrite forest_pred_reg; eauto.
+  - inv Heqo0. inv H. inv H2. constructor; intros; rewrite forest_exit_regs; auto.
+Qed.
+
+Lemma abstr_seq_reverse_correct_fold_inc :
+  forall sp instrs i0 i i' ti cf f' l p p' l' f preds preds' lm lm' ps',
+    (forall in_pred, PredIn in_pred p -> preds ! in_pred = Some tt) ->
+    (forall p : positive, preds ! p = None -> sem_pexpr (mk_ctx i0 sp ge) f #p p (is_ps i0) !! p) ->
+    valid_mem (is_mem i0) (is_mem i) ->
+    all_preds_in f preds ->
+    eval_predf (is_ps i) p = true ->
+    sem (mk_ctx i0 sp ge) f (i, None) ->
+    mfold_left update'_inc instrs (Some (p, f, l, lm)) = Some (p', f', l', lm') ->
+    mfold_left gather_predicates instrs (Some preds) = Some preds' ->
+    evaluable_pred_list (mk_ctx i0 sp ge) f'.(forest_preds) l' ->
+    evaluable_pred_list_m (mk_ctx i0 sp ge) f'.(forest_preds) lm' ->
+    sem_predset (mk_ctx i0 sp ge) f' ps' ->
+    sem (mk_ctx i0 sp ge) f' (i', Some cf) ->
+    state_lessdef i ti ->
+    evaluable_forest (mk_ctx i0 sp ge) f'.(forest_preds) f ->
+    exists ti',
+      SeqBB.step ge sp (Iexec ti) instrs (Iterm ti' cf)
+      /\ state_lessdef i' ti'.
+Proof.
+  induction instrs; intros * YPREDSIN YPREDNONE YVALID YALL YEVAL Y3 Y YGATHER Y0 YEVALUABLE YSEM_FINAL Y1 Y2 HEval.
+  - cbn in *. inv Y.
+    assert (X: similar {| ctx_is := i0; ctx_sp := sp; ctx_ge := ge |}
+                       {| ctx_is := i0; ctx_sp := sp; ctx_ge := ge |})
+      by reflexivity.
+    now eapply sem_det in X; [| exact Y1 | exact Y3 ].
+  - cbn -[update'_inc] in Y.
+    pose proof Y as YX.
+    apply OptionExtra.mfold_left_Some in YX. inv YX.
+    cbn in YGATHER.
+    pose proof YGATHER as YX.
+    apply OptionExtra.mfold_left_Some in YX. inv YX. rewrite H0 in YGATHER.
+    pose proof H0 as YGATHER_SINGLE. clear H0.
+    rewrite H in Y.
+    destruct x as ((p_mid & f_mid) & l_mid).
+    pose proof H as Hupdate'_inc.
+    unfold update'_inc, Option.bind2, Option.ret in H. repeat destr.
+    inv H.
+
+    destruct a.
+    + cbn in Heqo. inv Heqo. cbn in YGATHER_SINGLE. inv YGATHER_SINGLE.
+      exploit IHinstrs; eauto; simplify.
+      exists x; split; auto. econstructor. constructor. auto.
+    + exploit evaluable_pred_expr_exists_RBop; eauto.
+      eapply abstr_seq_revers_correct_fold_sem_pexpr_eval2_inc; eauto.
+      (* unfold evaluable_pred_list in Y0. eapply in_forest_evaluable; eauto. *)
+      inv YSEM_FINAL.
+      eapply eval_forest_update_inc; eauto.
+      unfold evaluable_pred_list. intros. eapply Y0.
+      eapply in_mfold_left_abstr_inc; eauto.
+      unfold evaluable_pred_list_m. intros. eapply YEVALUABLE.
+      eapply in_mfold_left_abstr_m_inc; eauto.
+      eapply gather_predicates_in_forest in YALL; eauto.
+      unfold all_preds_in in YALL. eauto.
+      intros [ti_mid HSTEP].
+
+      pose proof Y3 as YH.
+      pose proof HSTEP as YHSTEP.
+      pose proof Y2 as Y2SPLIT; inv Y2SPLIT.
+      eapply step_exists in YHSTEP.
+      2: { symmetry. econstructor; try eassumption; auto. }
+      inv YHSTEP. inv H1.
+      exploit sem_update_instr. auto. eauto. eauto. eauto. eauto. auto. intros.
+      exploit IHinstrs. 6: { eauto. } eapply gather_predicates_update_constant; eauto.
+      eapply update_rev_gather_constant; eauto.
+      unfold update', Option.bind2, Option.ret. rewrite Heqo; auto.
+      cbn in YVALID. transitivity m'; auto.
+      replace m' with (is_mem {| is_rs := rs; Gible.is_ps := ps; Gible.is_mem := m' |}) by auto.
+      eapply sem_update_valid_mem; eauto.
+      eapply gather_predicates_in_forest; eauto.
+      eapply eval_predf_update_true; eauto.
+      eauto. eauto. eauto. eauto. eauto. eauto. symmetry.
+      eapply state_lessdef_state_equiv; eauto.
+      inv YSEM_FINAL. eapply eval_forest_update_inc; eauto.
+      unfold evaluable_pred_list. intros. eapply Y0.
+      eapply in_mfold_left_abstr_inc; eauto.
+      unfold evaluable_pred_list_m. intros. eapply YEVALUABLE.
+      eapply in_mfold_left_abstr_m_inc; eauto.
+      intros [ti' [YHH HLD]].
+      exists ti'; split; eauto. econstructor; eauto.
+    + exploit evaluable_pred_expr_exists_RBload; eauto.
+      eapply abstr_seq_revers_correct_fold_sem_pexpr_eval2_inc; eauto.
+      inv YSEM_FINAL.
+      eapply eval_forest_update_inc; eauto.
+      unfold evaluable_pred_list. intros. eapply Y0.
+      eapply in_mfold_left_abstr_inc; eauto.
+      unfold evaluable_pred_list_m. intros. eapply YEVALUABLE.
+      eapply in_mfold_left_abstr_m_inc; eauto.
+      eapply gather_predicates_in_forest in YALL; eauto.
+      unfold all_preds_in in YALL. eauto.
+      intros [ti_mid HSTEP].
+
+      pose proof Y3 as YH.
+      pose proof HSTEP as YHSTEP.
+      pose proof Y2 as Y2SPLIT; inv Y2SPLIT.
+      eapply step_exists in YHSTEP.
+      2: { symmetry. econstructor; try eassumption; auto. }
+      inv YHSTEP. inv H1.
+      exploit sem_update_instr. auto. eauto. eauto. eauto. eauto. auto. intros.
+      exploit IHinstrs. 6: { eauto. } eapply gather_predicates_update_constant; eauto.
+      eapply update_rev_gather_constant; eauto.
+      unfold update', Option.bind2, Option.ret. rewrite Heqo; auto.
+      cbn in YVALID. transitivity m'; auto.
+      replace m' with (is_mem {| is_rs := rs; Gible.is_ps := ps; Gible.is_mem := m' |}) by auto.
+      eapply sem_update_valid_mem; eauto.
+      eapply gather_predicates_in_forest; eauto.
+      eapply eval_predf_update_true; eauto.
+      eauto. eauto. eauto. eauto. eauto. eauto. symmetry.
+      eapply state_lessdef_state_equiv; eauto.
+      inv YSEM_FINAL. eapply eval_forest_update_inc; eauto.
+      unfold evaluable_pred_list. intros. eapply Y0.
+      eapply in_mfold_left_abstr_inc; eauto.
+      unfold evaluable_pred_list_m. intros. eapply YEVALUABLE.
+      eapply in_mfold_left_abstr_m_inc; eauto.
+      intros [ti' [YHH HLD]].
+      exists ti'; split; eauto. econstructor; eauto.
+    + exploit evaluable_pred_expr_exists_RBstore; eauto.
+      eapply abstr_seq_revers_correct_fold_sem_pexpr_eval4_inc; eauto.
+
+      inv YSEM_FINAL.
+      eapply eval_forest_update_inc; eauto.
+      unfold evaluable_pred_list. intros. eapply Y0.
+      eapply in_mfold_left_abstr_inc; eauto.
+      unfold evaluable_pred_list_m. intros. eapply YEVALUABLE.
+      eapply in_mfold_left_abstr_m_inc; eauto.
+
+      eapply gather_predicates_in_forest in YALL; eauto.
+      unfold all_preds_in in YALL. eauto.
+      intros [ti_mid HSTEP].
+
+      pose proof Y3 as YH.
+      pose proof HSTEP as YHSTEP.
+      pose proof Y2 as Y2SPLIT; inv Y2SPLIT.
+      eapply step_exists in YHSTEP.
+      2: { symmetry. econstructor; try eassumption; auto. }
+      inv YHSTEP. inv H1.
+      exploit sem_update_instr. auto. eauto. eauto. eauto. eauto. auto. intros.
+      exploit IHinstrs. 6: { eauto. } eapply gather_predicates_update_constant; eauto.
+      eapply update_rev_gather_constant; eauto.
+      unfold update', Option.bind2, Option.ret. rewrite Heqo; auto.
+      cbn in YVALID. transitivity m'; auto.
+      replace m' with (is_mem {| is_rs := rs; Gible.is_ps := ps; Gible.is_mem := m' |}) by auto.
+      eapply sem_update_valid_mem; eauto.
+      eapply gather_predicates_in_forest; eauto.
+      eapply eval_predf_update_true; eauto.
+      eauto. eauto. eauto. eauto. eauto. eauto. symmetry.
+      eapply state_lessdef_state_equiv; eauto.
+
+      inv YSEM_FINAL. eapply eval_forest_update_inc; eauto.
+      unfold evaluable_pred_list. intros. eapply Y0.
+      eapply in_mfold_left_abstr_inc; eauto.
+      unfold evaluable_pred_list_m. intros. eapply YEVALUABLE.
+      eapply in_mfold_left_abstr_m_inc; eauto.
+
+      intros [ti' [YHH HLD]].
+      exists ti'; split; eauto. econstructor; eauto.
+    + exploit abstr_seq_revers_correct_fold_sem_pexpr_eval_inc.
+      2: { eauto. }
+      eapply update_rev_gather_constant; eauto.
+      unfold update', Option.bind2, Option.ret. rewrite Heqo; auto.
+      eauto.
+      eauto.
+      intros [ps_mid HPRED2].
+      exploit evaluable_pred_expr_exists_RBsetpred; eauto.
+      intros [ti_mid HSTEP].
+
+      pose proof Y3 as YH.
+      pose proof HSTEP as YHSTEP.
+      pose proof Y2 as Y2SPLIT; inv Y2SPLIT.
+      eapply step_exists in YHSTEP.
+      2: { symmetry. econstructor; try eassumption; auto. }
+      inv YHSTEP. inv H1.
+      exploit sem_update_instr. auto. eauto. eauto. eauto. eauto. auto. intros.
+      exploit IHinstrs. 6: { eauto. } eapply gather_predicates_update_constant; eauto.
+      eapply update_rev_gather_constant; eauto.
+      unfold update', Option.bind2, Option.ret. rewrite Heqo; auto.
+      cbn in YVALID. transitivity m'; auto.
+      replace m' with (is_mem {| is_rs := rs; Gible.is_ps := ps; Gible.is_mem := m' |}) by auto.
+      eapply sem_update_valid_mem; eauto.
+      eapply gather_predicates_in_forest; eauto.
+      eapply eval_predf_update_true; eauto.
+      eauto. eauto. eauto. eauto. eauto. eauto. symmetry.
+      eapply state_lessdef_state_equiv; eauto.
+
+      inv YSEM_FINAL. eapply eval_forest_update_inc; eauto.
+      unfold evaluable_pred_list. intros. eapply Y0.
+      eapply in_mfold_left_abstr_inc; eauto.
+      unfold evaluable_pred_list_m. intros. eapply YEVALUABLE.
+      eapply in_mfold_left_abstr_m_inc; eauto.
+
+      intros [ti' [YHH HLD]].
+      exists ti'; split; eauto. econstructor; eauto.
+    + case_eq (eval_predf (is_ps i) (dfltp o)); intros.
+      * exploit evaluable_pred_expr_exists_RBexit2; eauto; intros HSTEP.
+        instantiate (1:=c) in HSTEP.
+        instantiate (1:=sp) in HSTEP.
+        exploit evaluable_pred_expr_exists_RBexit3. eauto. eauto. intros.
+        pose proof (state_lessdef_state_equiv i ti). inv H1.
+        specialize (H2 Y2).
+        pose proof (step_exists_Iterm ge sp ti _ i _ HSTEP
+                      ltac:(symmetry; assumption)).
+        exploit sem_update_instr_term; eauto; intros. inv H4.
+        exploit abstr_fold_falsy; auto. eauto. eapply equiv_update_inc; eauto. cbn. auto.
+        intros. eapply sem_det in Y1; eauto. inv Y1. inv H7.
+        eexists. split. constructor. eauto. transitivity i.
+        symmetry; auto. auto. reflexivity.
+      * exploit evaluable_pred_expr_exists_RBexit; eauto; intros HSTEP.
+        instantiate (1:=c) in HSTEP. instantiate (1:=sp) in HSTEP.
+        pose proof Y3 as YH.
+        pose proof HSTEP as YHSTEP.
+        pose proof Y2 as Y2SPLIT; inv Y2SPLIT.
+        eapply step_exists in YHSTEP.
+        2: { symmetry. econstructor; try eassumption; auto. }
+        inv YHSTEP. inv H2.
+        exploit sem_update_instr. auto. eauto. eauto. eauto. eapply Heqo. eauto. auto. intros.
+        exploit IHinstrs. 6: { eauto. } eapply gather_predicates_update_constant; eauto.
+        eapply update_rev_gather_constant; eauto.
+        unfold update', Option.bind2, Option.ret. rewrite Heqo; auto.
+        cbn in YVALID. transitivity m'; auto.
+        replace m' with (is_mem {| is_rs := rs; Gible.is_ps := ps; Gible.is_mem := m' |}) by auto.
+        cbn. inv H4.
+        reflexivity.
+        eapply gather_predicates_in_forest; eauto.
+        eapply eval_predf_update_true; eauto.
+        eauto. eauto. eauto. eauto. eauto. eauto. symmetry.
+        eapply state_lessdef_state_equiv; eauto.
+
+      inv YSEM_FINAL. eapply eval_forest_update_inc; eauto.
+      unfold evaluable_pred_list. intros. eapply Y0.
+      eapply in_mfold_left_abstr_inc; eauto.
+      unfold evaluable_pred_list_m. intros. eapply YEVALUABLE.
+      eapply in_mfold_left_abstr_m_inc; eauto.
+
+        intros [ti' [YHH HLD]].
+        exists ti'; split; eauto. econstructor; eauto.
+        Unshelve. all: exact nil.
+Qed.
+
 Lemma sem_empty :
   forall G (ctx: @Abstr.ctx G),
     sem ctx empty (ctx_is ctx, None).
@@ -1832,6 +2494,32 @@ Proof.
     try eassumption; try reflexivity; auto using sem_empty, all_preds_in_empty.
   inversion 1.
   intros; repeat constructor.
+Qed.
+
+Lemma abstr_seq_reverse_correct_inc:
+  forall sp x i i' ti cf x' l lm,
+    abstract_sequence'_inc x = Some (x', l, lm) ->
+    evaluable_pred_list (mk_ctx i sp ge) x'.(forest_preds) l ->
+    evaluable_pred_list_m (mk_ctx i sp ge) x'.(forest_preds) lm ->
+    sem (mk_ctx i sp ge) x' (i', (Some cf)) ->
+    state_lessdef i ti ->
+   exists ti', SeqBB.step ge sp (Iexec ti) x (Iterm ti' cf)
+           /\ state_lessdef i' ti'.
+Proof.
+  intros. unfold abstract_sequence'_inc in H.
+  unfold Option.map, Option.bind in H. repeat destr. inv H. inv Heqo.
+  pose proof H2 as X. inv X.
+  eapply abstr_seq_reverse_correct_fold_inc;
+    try eassumption; try reflexivity; auto using sem_empty, all_preds_in_empty.
+  inversion 1.
+  intros; repeat constructor.
+  unfold evaluable_forest; split.
+  - intros. unfold "#r". cbn. rewrite RTree.gempty. 
+    unfold evaluable_pred_expr. eexists. constructor. constructor.
+    constructor.
+  - intros. unfold "#r". cbn. rewrite RTree.gempty. 
+    unfold evaluable_pred_expr_m. eexists. constructor. constructor.
+    constructor.
 Qed.
 
 (*|
